aeneas-lean/Tree.lean
@@ -179,3 +179,4 @@ import Tree.BulkUpdate.Success
 import Tree.BulkUpdate.Contents
 import Tree.ProgressiveTree.Rebase.Soundness
 import Tree.ProgressiveList.Rebase.Pointer
+import Tree.Rebase.HashShortcutSteps
